Define a transformation that applies an arbitrary transformation below the outermost CLetMut and prove the soundness preservation

fiat2/src/fiat2/IndexTransf.v
@@ -168,6 +168,39 @@ Section WithMap.
     Notation value := (value (width:=width)).
     Context {locals : map.map string value} {locals_ok : map.ok locals}.
 
+    Definition apply_below_letmut f (Gstore Genv : tenv) (c : command) :=
+      match c with
+      | CLetMut e x c' =>
+          match synthesize_expr Gstore Genv e with
+          | Success (t, _) => CLetMut e x (f (map.put Gstore x t) Genv c')
+          | Failure _ => c
+          end
+      | _ => c
+      end.
+
+    Lemma apply_below_letmut_sound : forall f,
+        transf_sound (locals:=locals) f ->
+        transf_sound (locals:=locals) (apply_below_letmut f).
+    Proof.
+      unfold transf_sound; intros.
+      destruct c; auto; cbn.
+      repeat (case_match; auto).
+      apply typechecker_sound in E as H_ty; auto.
+      invert_well_typed.
+      eapply synthesizable_ty_unique in E as E'; eauto; subst.
+      intuition idtac.
+      1:{ econstructor; eauto.
+          apply H; auto.
+          eapply tenv_wf_step, type_of__type_wf;
+            [ | | | eauto ]; assumption. }
+      1:{ eapply H in H7; eauto; intuition idtac.
+          1:{ cbn. rewrite H8; auto.
+              apply locals_wf_step;
+                eauto using type_sound. }
+          eapply tenv_wf_step, type_of__type_wf;
+            [ | | | eauto ]; assumption. }
+    Qed.
+
     Section WithIndex.
       Context {idx : IndexInterface.index} {idx_wf : value -> value -> Prop} {idx_ok : ok idx idx_wf}.
       Context (id_tag aux_tag: string).
@@ -924,6 +957,7 @@ End WithMap.
 Ltac apply_transf_sound_lemmas :=
   lazymatch goal with
   | |- transf_sound (apply_idx_related_transfs _ _ _) => apply apply_idx_related_transfs_sound
+  | |- transf_sound (apply_below_letmut _) => apply apply_below_letmut_sound
   | |- aug_transf_sound _ _ _ (fun _ => Basics.compose _ _) => apply aug_transf_sound_compose
   | |- transf_sound (fun _ _ => Basics.compose _ _) => apply transf_sound_compose
   | |- aug_transf_sound _ _ _ (fun _ => repeat_transf _ _) => apply repeat_transf_preserve_aug_transf_sound
